Update RequestBlood.dfy

dafny/RequestBlood.dfy
@@ -74,11 +74,26 @@ reads set x | x in a[..];
     ==> a[k].use_by_date <= a[j].use_by_date)
 }
 
-method BubbleSortExpiration(a: array<Blood>, asc: bool)
+function count ( a : seq <Blood > , v : int) : nat
+reads a
+{
+    if (| a | > 0) then
+        if( a [0].blood_id == v ) then 1 + count ( a [1..] , v )
+        else count ( a [1..] , v )
+    else 0
+}
+
+predicate permutation ( a : seq <Blood > , b : seq <Blood >)
+{
+    forall v :: count (a , v ) == count (b , v )
+}
+
+method BubbleSortExpiration(a: array<Blood>, asc: bool) returns (sorted: array<Blood>)
 requires a != null;
 requires forall j :: 0 <= j < a.Length ==> a[j] != null && a[j].Valid();
 ensures forall j :: 0 <= j < a.Length ==> a[j] != null && a[j].Valid();
 ensures SortedExpiration(a, asc);
+ensures permutation (a[..],old(a[..]))
 modifies a;
 {
   var i := a.Length - 1;
@@ -118,6 +133,7 @@ modifies a;
 
     i := i - 1;
   }
+  sorted := a;
 }
 
 method hasEnoughVolume(blood: seq<Blood>, volume: int) returns (b: bool)
@@ -129,8 +145,10 @@ method hasEnoughVolume(blood: seq<Blood>, volume: int) returns (b: bool)
     totalVolume := 0;
 
     while i < |blood|
+    decreases |blood| - i
     {
         totalVolume := totalVolume + blood[i].volume;
+        i := i + 1;
     }
 
     if totalVolume > volume {
@@ -139,18 +157,30 @@ method hasEnoughVolume(blood: seq<Blood>, volume: int) returns (b: bool)
 }
 
 method requestBlood(allBlood: seq<Blood>, bt: BloodType, amount: int, deliverByDate: int) returns (order: seq<Blood>)
+requires forall i :: 0 <= i < |allBlood| ==> allBlood[i].Valid();
+ensures forall j :: 0 <= j < |order| ==> order[j] != null
+ensures forall j :: 0 <= j < |order| ==> order[j].blood_type == bt
+ensures forall j :: 0 <= j < |order| ==> order[j].use_by_date <= deliverByDate
 {
     var i: int;
     i := 0;
     var suitable : seq<Blood>;
     suitable := [];
+
     while i < |allBlood|
+    decreases |allBlood| - i
+    invariant 0 <= i <= |allBlood|;
+    invariant forall j :: 0 <= j < |suitable| ==> suitable[j] != null && suitable[j].Valid();
+    invariant forall j :: 0 <= j < |suitable| ==> suitable[j].suitablity == true && suitable[j].use_by_date <= deliverByDate && suitable[j].blood_type == bt
     {
-        if allBlood[i].suitablity == true && allBlood[i].use_by_date < deliverByDate && allBlood[i].blood_type == bt
+        if allBlood[i].suitablity == true && allBlood[i].use_by_date <= deliverByDate && allBlood[i].blood_type == bt
         {
-            suitable := suitable + allBlood[i..i+1];
+            assert allBlood[i].Valid();
+            suitable := suitable + [allBlood[i]];
         }
+        i := i + 1;
     }
+    
     var check : bool;
     check := hasEnoughVolume(suitable, amount);
     if !check{
@@ -159,14 +189,38 @@ method requestBlood(allBlood: seq<Blood>, bt: BloodType, amount: int, deliverByD
     }
     var True: bool;
     True := true;
-    suitable := BubbleSortExpiration(suitable);
+
+    var suitableArray: array<Blood>;
+    suitableArray := new Blood[|suitable|](i requires 0 <= i < |suitable| reads suitable => suitable[i]);
+    i := 0;
+    while (i < |suitable|)
+        decreases |suitable| - i
+        invariant 0 <= i <= |suitable|;
+        invariant forall j :: 0 <= j < |suitable| ==> suitable[j] != null && suitable[j].Valid();
+        invariant forall j :: 0 <= j < i ==> suitableArray[j] != null && suitableArray[j].Valid();
+        invariant forall j :: 0 <= j < suitableArray.Length ==> suitableArray[j].suitablity == true && suitableArray[j].use_by_date <= deliverByDate && suitableArray[j].blood_type == bt
+    {
+        suitableArray[i] := suitable[i];
+        i := i + 1;
+        assert suitableArray[i - 1] != null && suitableArray[i - 1].Valid();
+    }
+    
+    //forall i | 0 <= i && i < suitableArray.Length { suitableArray[i] := suitable[i] ; }
+    
+    suitableArray := BubbleSortExpiration(suitableArray, True);
+    assert forall j :: 0 <= j < suitableArray.Length ==> suitableArray[j].suitablity == true && suitableArray[j].use_by_date <= deliverByDate && suitableArray[j].blood_type == bt;
+    suitable := suitableArray[0..suitableArray.Length];
     order := [];
     i := 0;
     while i < |suitable|
+    decreases |suitable| - i
+    invariant forall j :: 0 <= j < |suitable| ==> suitable[j].suitablity == true && suitable[j].use_by_date <= deliverByDate && suitable[j].blood_type == bt
+    invariant forall j :: 0 <= j < |order| ==> order[j].suitablity == true && order[j].use_by_date <= deliverByDate && order[j].blood_type == bt
     {
         check := hasEnoughVolume(order, amount);
         if !check{
             order := order + suitable[i..i+1];
         }
+        i := i + 1;
     }
 }
